examples/ghc/manual/Panic.v
@@ -26,3 +26,6 @@ Parameter panic : forall {a} `{Default a}, String -> a.
 Parameter sorry : forall {a} `{Default a}, String -> a.
 Parameter pgmError : forall {a} `{Default a}, String -> a.
 Parameter warnPprTrace :  forall {a}, bool -> String -> Integer -> String -> a -> a.
+
+Parameter assertPanic :  forall {a} `{Default a}, String -> Integer -> a.
+Parameter assertPprPanic : forall {a} `{Default a}, String -> Integer -> String -> String -> a.
